theorems: implement `opt` and `⟨⟨func⟩⟩`

programs/mean_s32/eclass.lean
@@ -1,12 +1,13 @@
 import theorems.iN
 
 import Lean
+import Qq
+
+open Qq
 open Lean Parser Elab Meta Tactic
 
-def root₁ (x y : iN 32) := (x +nsw y) >>>ₛ 1
 def root₂ (x y : iN 32) := (x +nsw y) /ₛ 2
 
-#eval (root₁ 100 50)
 #eval (root₂ 100 50)
 
 theorem comm (x y : iN 32) : x +nsw y ~> y +nsw x := by
@@ -15,19 +16,26 @@ theorem comm (x y : iN 32) : x +nsw y ~> y +nsw x := by
   all_goals simp [simp_iN]
   bv_decide
 
+theorem commw (x y : iN 32) : x + y ~> y + x := by
+  cases x
+  cases y
+  all_goals simp [simp_iN]
+  ac_nf
+
 theorem rewrite_test₁ (x y : iN 32) : x +nsw y + 1 ~> y +nsw x + 1 := by
   exact Rewrite.congrApp (fun x => x + 1) (by simp [simp_iN]) (comm x y)
 
 theorem rewrite_test₂ (x y : iN 32) : x +nsw y + 1 ~> y +nsw x + 1 := by
-  apply_rw comm
+  opt_rw comm
 
-/-
-partial def elabRoot : Syntax → MetaM Expr
- -/
-elab "⟨⟨" func:term "⟩⟩" : term => do
-  let func ← Term.elabTerm func none
+-- given some expr, optimise to expr' with proof that expr ~> expr'
+set_option trace.Meta.opti true
 
-  dbg_trace func
-  return func
+def root₁ (x y : iN 32) := x +nsw y
+def root := ⟨⟨root₁⟩⟩ -- "optimise" `root₁`
 
-def root := ⟨⟨root₁⟩⟩
+/- basically, the only "optimisation" done right now turns every `x ~> x + 0` -/
+example : root = fun x y => x +nsw y := by rfl
+
+theorem opt_works (x y : iN 32) : root₁ x y ~> root x y := by
+  opt_showcorrect root₁ root
