theorems/iN/tactics/iN_opt.lean
@@ -1,0 +1,61 @@
+import Lean
+import theorems.iN.iN_def
+import theorems.iN.iN_rewrite
+import theorems.iN.tactics.shared
+
+open Lean Elab Tactic Meta Command
+
+structure OptState where
+  -- TODO memo
+  -- lhs ~> rhs
+  rewrites : Array Expr
+deriving Inhabited
+
+abbrev OptM := StateRefT OptState MetaM
+
+structure OptResult where
+  /-- The simplified version of `e` -/
+  expr : Expr
+  /-- A proof that `$e ~> $expr`, where the simplified expression is on the RHS.
+  If `none`, the proof is assumed to be `Rewrite.refl`. -/
+  proof? : Option Expr := none
+deriving Inhabited
+
+abbrev OptProc := Expr → OptM (Option OptResult)
+
+syntax (name := optProcPattern) "optproc% " term " => " ident : command
+/--
+A user-defined optimisation procedure used by the `opt` tactic, and its variants.
+-/
+syntax (docComment)? attrKind "optproc " ident " (" term ")" " := " term : command
+/--
+A user-defined optimisation procedure declaration. To activate this procedure in `opt` tactic,
+we must provide it as an argument, or use the command `attribute` to set its `[opt]` attribute.
+-/
+syntax (docComment)? "optproc_decl " ident " (" term ")" " := " term : command
+
+macro_rules
+  | `($[$doc?:docComment]? optproc_decl $n:ident ($pattern:term) := $body) => do
+    let simprocType := `OptProc
+    `($[$doc?:docComment]? def $n:ident : $(mkIdent simprocType) := $body
+      optproc% $pattern => $n)
+
+macro_rules
+  | `($[$doc?:docComment]? $_:attrKind optproc $n:ident ($pattern:term) := $body) => do
+     return mkNullNode <|
+       #[(← `($[$doc?:docComment]? optproc_decl $n ($pattern) := $body))]
+
+def checkOptprocType (declName : Name) : CoreM Bool := do
+  let decl ← getConstInfo declName
+  match decl.type with
+  | .const ``OptProc _ => pure false
+  | _ => throwError "unexpected type at '{declName}', 'Optproc' expected"
+
+@[command_elab optProcPattern]
+def elabOptprocPattern : CommandElab := fun stx => do
+  let `(optproc% $pattern => $declName) := stx | throwUnsupportedSyntax
+  liftTermElabM do
+    let declName ← realizeGlobalConstNoOverload declName
+    discard <| checkOptprocType declName
+    let keys ← elabSimprocKeys pattern
+    registerOptProc declName keys
