theorems/iN/tactics/iN_tactic_opt.lean
@@ -1,0 +1,181 @@
+import Lean
+import theorems.iN.iN_def
+import theorems.iN.iN_llvm
+import theorems.iN.iN_lemmas
+import theorems.iN.iN_rewrite
+
+import theorems.iN.tactics.shared
+import theorems.iN.tactics.iN_opt
+
+open Lean Elab Tactic Meta
+
+def isiNType (e : Expr) : MetaM Bool := do
+  let eType ← inferType e
+  let eType ← whnf eType
+  if let .const name _ := eType.getAppFn then
+    return name == ``iN
+  return false
+
+def getiNBitWidth (e : Expr) : MetaM Expr := do
+  let eType ← inferType e
+  let eType ← whnf eType
+  match_expr eType with
+  | iN w => return w
+  | _ => throwError "expected iN type, got {eType}"
+
+def getiNBitWidthFromType (ty : Expr) : MetaM Expr := do
+  let ty ← whnf ty
+  match_expr ty with
+  | iN w => return w
+  | _ => throwError "expected iN type, got {ty}"
+
+namespace OptM
+
+def runOptM (x : OptM α) : MetaM α :=
+  x.run' default
+
+def handleOpt (expr : Expr) : OptM $ Option OptResult := do
+  return none
+  --return { expr, proof? := none }
+  /- let bw : Q(Nat) ← getiNBitWidth expr
+  let expr : Q(iN $bw) := expr
+
+  let zero : Q(iN $bw) := q(0)
+  let newExpr := q($expr + $zero)
+  let proof := q(Rewrite.add_zero $expr)
+
+  return { expr := newExpr, proof? := some proof } -/
+
+def handleSingleRewrite (abstract : Expr) (hole : Expr) : OptM Expr := do
+  /- try optimising, or do nothing -/
+  let some optResult ← handleOpt hole
+    | return hole
+
+  let bw ← getiNBitWidth hole
+  let α := (Expr.app (.const `iN []) bw)
+
+  let proof ←
+    match optResult.proof? with
+    | some p => pure p
+    | none   => pure (mkAppN (mkConst ``Rewrite.refl) #[bw, hole])
+
+  -- optResult.proof : hole ~> optResult.expr
+  -- ⊢ abstract hole ~> abstract optResult.expr
+  let motive := Lean.mkLambda `_a BinderInfo.default α abstract
+  let motive_wf ← proveCongruence motive bw
+  let congrProof ← mkAppM ``Rewrite.congrApp #[motive, motive_wf, proof]
+
+  trace[Meta.opti] m!"rewrite {hole} ~> {optResult.expr} by {proof}"
+
+  -- append proof to state
+  modify fun s => { s with rewrites := s.rewrites.push congrProof }
+  return optResult.expr
+
+def proveRewrites : OptM $ Option Expr := do
+  let st ← get
+  if st.rewrites.isEmpty then
+    return none
+
+  let mut finalProof := st.rewrites[0]!
+  for proof in st.rewrites[1:] do
+    finalProof ← mkAppM ``Rewrite.trans #[finalProof, proof]
+
+  return some finalProof
+
+end OptM
+
+
+structure RewriteSite where
+  /-- The expression with a subterm replaced by a bound variable `#0`.
+      In this single-pass model, this is the *local* abstract, not the global one. -/
+  abstract : Expr
+  /-- The subterm that was replaced by the hole (`#0`). -/
+  filler   : Expr
+  deriving Inhabited
+
+partial def walkAndTransform (e : Expr) : OptM Expr := do
+  /- let cache ← IO.mkRef (α := Std.HashMap Expr Expr) {} -/
+
+  let rec traverse (subExpr : Expr) (context : Expr → MetaM Expr) : OptM Expr := do
+    /- if let some cachedResult := (← cache.get).get? subExpr then
+      return (← context (← instantiateMVars cachedResult)) -/
+
+    let rebuiltExpr ← match subExpr with
+    | .app .. => do
+      /- handle full applications as a single unit -/
+      let fn := subExpr.getAppFn
+      let args := subExpr.getAppArgs
+
+      let mut args' := #[]
+      for i in [:args.size] do
+        let mut arg := args[i]!
+
+        /- only process an argument if it is of type iN -/
+        if !(arg.isLit || arg.isConst) && (← isiNType arg) then
+          arg ← traverse arg (fun hole => context (mkAppN fn (args'.push hole ++ args.extract (i+1) args.size)))
+
+        args' := args'.push arg
+
+      pure $ mkAppN fn args'
+    | .mdata _ i => traverse i context
+    | _ => pure subExpr
+
+    /- TODO we don't expect let binds or (definitely) lambdas in here -/
+    let abstract ← context (mkBVar 0)
+    let finalExpr ← OptM.handleSingleRewrite abstract rebuiltExpr
+
+    /- cache.modify (·.insert subExpr finalExpr) -/
+    return finalExpr
+
+  traverse e (fun hole => pure hole)
+
+elab "⟨⟨" func:term "⟩⟩" : term => do
+  let func ← Term.elabTerm func none
+  let func ← unfoldDefinition func
+
+  let expr ← lambdaTelescope func fun xs A => OptM.runOptM do
+    let B ← walkAndTransform A
+    mkLambdaFVars xs B
+
+  return expr
+
+/-- On a goal of `lhs ~> rhs`, repeatedly apply rewrites to transform the goal into `lhs' ~> rhs`.  -/
+elab "opti" : tactic => withMainContext do
+  let mvarId ← getMainGoal
+  mvarId.checkNotAssigned `opt
+
+  let e ← getMainTarget
+  let e ← instantiateMVars e
+
+  -- lhs ~> rhs
+  let (_, lhs, rhs) ← match_expr e with
+  | Rewrite n lhs rhs => pure (n, lhs, rhs)
+  | _ => throwTacticEx `opt_rewrite mvarId m!"not a rewrite{indentExpr e}"
+
+  let newGoal ← OptM.runOptM do
+    let lhs' ← walkAndTransform lhs
+    let some proof ← OptM.proveRewrites
+      | throwTacticEx `opt mvarId "no rewrites were performed"
+
+    -- Rewrite.trans (lhs ~> lhs') (lhs' ~> rhs) (lhs ~> rhs)
+    --                             ^^^^^^^^^^^^^ create a new metavariable/goal
+
+    trace[Meta.opti] m!"final proof term {proof}"
+
+    let newGoalType ← mkAppM ``Rewrite #[lhs', rhs]
+    let newGoalMVar ← mkFreshExprMVar (some newGoalType)
+    let fullProof ← mkAppM ``Rewrite.trans #[proof, newGoalMVar]
+    mvarId.assign fullProof
+
+    pure newGoalMVar.mvarId!
+
+  replaceMainGoal [newGoal]
+
+macro "opt " : tactic =>
+  `(tactic| (opti; try (with_reducible rfl)))
+
+macro "opt_showcorrect " lhs:ident rhs:ident : tactic =>
+  `(tactic| (unfold $lhs $rhs; solve
+    | try (with_reducible rfl)
+    | opti; try (with_reducible rfl)
+  ))
