theorems/iN/tactics/shared.lean
@@ -1,0 +1,75 @@
+import Lean
+import theorems.iN.iN_def
+import theorems.iN.iN_rewrite
+
+open Lean Elab Tactic Meta
+
+/- set_option trace.Meta.opti true -/
+initialize registerTraceClass `Meta.opti
+
+structure OptProcDecl where
+  declName : Name
+  keys     : Array SimpTheoremKey
+deriving Inhabited
+
+structure OptProcDeclExtState where
+  entries : PHashMap Name (Array SimpTheoremKey) := {}
+deriving Inhabited
+
+def OptProcDecl.lt (decl₁ decl₂ : OptProcDecl) : Bool :=
+  Name.quickLt decl₁.declName decl₂.declName
+
+initialize optProcDeclExt : PersistentEnvExtension OptProcDecl OptProcDecl OptProcDeclExtState ←
+  registerPersistentEnvExtension {
+    mkInitial       := return { entries := {} }
+    addImportedFn   := fun _ => return { entries := {} }
+    addEntryFn      := fun s d => { s with entries := s.entries.insert d.declName d.keys }
+    exportEntriesFn := fun s =>
+      let result := s.entries.foldl (init := #[]) fun result declName keys => result.push { declName, keys }
+      result.qsort OptProcDecl.lt
+  }
+
+def getOptProcDeclKeys? (declName : Name) : CoreM (Option (Array SimpTheoremKey)) := do
+  let env ← getEnv
+  let keys? ← match env.getModuleIdxFor? declName with
+    | some modIdx => do
+      let some decl := (optProcDeclExt.getModuleEntries env modIdx).binSearch { declName, keys := #[] } OptProcDecl.lt
+        | pure none
+      pure (some decl.keys)
+    | none        => pure ((optProcDeclExt.getState env).entries.find? declName)
+  if let some keys := keys? then
+    return some keys
+  else
+    return none
+
+def isOptProc (declName : Name) : CoreM Bool :=
+  return (← getOptProcDeclKeys? declName).isSome
+
+def registerOptProc (declName : Name) (keys : Array SimpTheoremKey) : CoreM Unit := do
+  let env ← getEnv
+  unless (env.getModuleIdxFor? declName).isNone do
+    throwError "invalid optProc declaration '{declName}', function declaration is in an imported module"
+  if (← isOptProc declName) then
+    throwError "invalid optProc declaration '{declName}', it has already been declared"
+  modifyEnv fun env => optProcDeclExt.modifyState env fun s => { s with entries := s.entries.insert declName keys }
+
+/- Proves `f poison = poison`. -/
+def proveCongruence (motive : Expr) (n : Expr) : MetaM Expr := do
+  let poison := mkApp (.const ``poison []) n
+  let poison_app := mkApp motive poison
+  let goalType ← mkEq poison_app poison
+
+  let proofMVar ← mkFreshExprMVar goalType .synthetic `h_cong_proof
+
+  let ctx ← Simp.mkContext
+    (config := { beta := true })
+    (simpTheorems := #[← getSimpTheorems, ← iNInst.getTheorems])
+    (congrTheorems := (← getSimpCongrTheorems))
+  let (result?, _) ← simpGoal proofMVar.mvarId! ctx
+
+  if let some _ := result? then
+    /- throwTactic `opt_rewrite x
+      m!"unable to prove congruence goal `motive poison = poison` automatically with `simp [simp_iN]`" -/
+    throwError "unable to prove congruence goal `motive poison = poison` automatically with `simp [simp_iN]`"
+
+  instantiateMVars proofMVar
