theorems/iN_denote/iNExpr.lean
@@ -1,0 +1,66 @@
+import theorems.iN
+
+inductive iNBinOp where
+  | add
+  | addNsw
+  | addNuw
+  | addNw
+deriving Hashable, DecidableEq, Repr
+
+namespace iNBinOp
+
+def eval : iNBinOp → (iN w → iN w → iN w)
+  | .add => iN.add
+  | .addNsw => iN.addNsw
+  | .addNuw => iN.addNuw
+  | .addNw => iN.addNw
+
+end iNBinOp
+
+inductive iNExpr : Nat → Type where
+  | poison : iNExpr n
+  | const : (value : Nat) → iNExpr n
+  | input : (idx : Nat) → iNExpr n
+  | binop : iNBinOp → iNExpr n → iNExpr n → iNExpr n
+with
+  @[computed_field]
+  hashCode : (n : Nat) → iNExpr n → UInt64
+    | n, .poison => mixHash 3 (hash n)
+    | n, .input idx => mixHash 5 $ mixHash (hash n) (hash idx)
+    | n, .const value => mixHash 7 $ mixHash (hash n) (hash value)
+    | n, .binop op lhs rhs => mixHash 11 $ mixHash (hash op) $ mixHash (lhs.hashCode) (rhs.hashCode)
+deriving DecidableEq, Repr, Inhabited
+
+instance : Hashable $ iNExpr n where
+  hash n := n.hashCode
+
+/- instance decEq : DecidableEq (iNExpr n) := fun l r =>
+  withPtrEqDecEq l r fun _ =>
+    if h : hash l ≠ hash r then
+      .isFalse (ne_of_apply_ne hash h)
+    else
+      ... -/
+
+namespace iNExpr
+
+structure PackediN where
+  n : Nat
+  expr : iN n
+
+abbrev Assignment := Lean.RArray PackediN
+
+def Assignment.get (assign : Assignment) (idx : Nat) : PackediN :=
+  Lean.RArray.get assign idx
+
+def eval (assign : Assignment) : iNExpr n → iN n
+  | .const v => iN.bitvec v
+  | .input idx =>
+    let pack := assign.get idx
+    if h : pack.n = n then
+      h ▸ pack.expr
+    else
+      panic! "type mismatch {pack.n} != {n}"
+  | .binop op lhs rhs => (op.eval) (eval assign lhs) (eval assign rhs)
+  | .poison => iN.poison
+
+end iNExpr
